spec/sail/lean/Out.lean
@@ -25,7 +25,7 @@ open LogicalOp
 open CompareOp
 open BarrierExecutionTarget
 
-/-- Type quantifiers: k_ex18464_ : Bool, k_ex18463_ : Bool -/
+/-- Type quantifiers: k_ex21856_ : Bool, k_ex21855_ : Bool -/
 def neq_bool (x : Bool) (y : Bool) : Bool :=
   (! (x == y))
 
@@ -175,7 +175,7 @@ def ConditionHolds (cond : (BitVec 4)) (nzcv : (BitVec 4)) : Bool :=
   then (! result)
   else result
 
-/-- Type quantifiers: k_ex18648_ : Bool, k_ex18647_ : Bool, k_datasize : Nat, k_datasize ∈
+/-- Type quantifiers: k_ex22040_ : Bool, k_ex22039_ : Bool, k_datasize : Nat, k_datasize ∈
   {32, 64} -/
 def integer_conditional_select (condition : (BitVec 4)) (nzcv : (BitVec 4)) (else_inc : Bool) (else_inv : Bool) (operand1 : (BitVec k_datasize)) (operand2 : (BitVec k_datasize)) : (BitVec k_datasize) :=
   let result : (BitVec k_datasize) := operand2
@@ -191,7 +191,7 @@ def integer_conditional_select (condition : (BitVec 4)) (nzcv : (BitVec 4)) (els
     then (BitVec.addInt result 1)
     else result)
 
-/-- Type quantifiers: k_ex18664_ : Bool, k_datasize : Nat, k_datasize ∈ {32, 64} -/
+/-- Type quantifiers: k_ex22056_ : Bool, k_datasize : Nat, k_datasize ∈ {32, 64} -/
 def integer_conditional_compare_register (condition : (BitVec 4)) (nzcv : (BitVec 4)) (flags__arg : (BitVec 4)) (operand1 : (BitVec k_datasize)) (operand2__arg : (BitVec k_datasize)) (sub_op : Bool) : (BitVec 4) :=
   let flags : (BitVec 4) := flags__arg
   let operand2 : (BitVec k_datasize) := operand2__arg
@@ -336,7 +336,7 @@ def vector_transfer_integer_dup (datasize : Nat) (elements : Nat) (esize : Nat) 
     loop_vars := (aset_Elem result e esize element)
   (pure loop_vars)
 
-/-- Type quantifiers: k_ex18803_ : Bool, datasize : Nat, elements : Nat, esize : Nat, esize ≥ 1
+/-- Type quantifiers: k_ex22195_ : Bool, datasize : Nat, elements : Nat, esize : Nat, esize ≥ 1
   ∧ elements ≥ 1 ∧ (elements * esize) = datasize -/
 def vector_arithmetic_binary_uniform_add_wrapping_single (datasize : Nat) (elements : Nat) (esize : Nat) (operand1 : (BitVec datasize)) (operand2 : (BitVec datasize)) (sub_op : Bool) : (BitVec datasize) := Id.run do
   let result : (BitVec datasize) := (Zeros datasize)
@@ -359,7 +359,7 @@ def vector_arithmetic_binary_uniform_add_wrapping_single (datasize : Nat) (eleme
     (pure loop_vars) ) : Id ((BitVec esize) × (BitVec esize) × (BitVec datasize)) )
   (pure result)
 
-/-- Type quantifiers: k_ex18871_ : Bool, k_ex18870_ : Bool, datasize : Nat, elements : Nat, esize :
+/-- Type quantifiers: k_ex22263_ : Bool, k_ex22262_ : Bool, datasize : Nat, elements : Nat, esize :
   Nat, esize ≥ 1 ∧ elements ≥ 1 ∧ (elements * esize) = datasize -/
 def vector_arithmetic_binary_uniform_maxmin_single (datasize : Nat) (elements : Nat) (esize : Nat) (operand1 : (BitVec datasize)) (operand2 : (BitVec datasize)) (minimum : Bool) (is_unsigned : Bool) : (BitVec datasize) := Id.run do
   let result : (BitVec datasize) := (Zeros datasize)
@@ -384,7 +384,7 @@ def vector_arithmetic_binary_uniform_maxmin_single (datasize : Nat) (elements : 
     (pure loop_vars) ) : Id (Int × Int × Int × (BitVec datasize)) )
   (pure result)
 
-/-- Type quantifiers: k_ex18922_ : Bool, k_ex18921_ : Bool, datasize : Nat, elements : Nat, esize :
+/-- Type quantifiers: k_ex22314_ : Bool, k_ex22313_ : Bool, datasize : Nat, elements : Nat, esize :
   Nat, esize ≥ 1 ∧ elements ≥ 1 ∧ (elements * esize) = datasize -/
 def vector_arithmetic_binary_uniform_cmp_int (cmp_eq : Bool) (datasize : Nat) (elements : Nat) (esize : Nat) (operand1 : (BitVec datasize)) (operand2 : (BitVec datasize)) (is_unsigned : Bool) : (BitVec datasize) := Id.run do
   let result : (BitVec datasize) := (Zeros datasize)
@@ -413,7 +413,7 @@ def vector_arithmetic_binary_uniform_cmp_int (cmp_eq : Bool) (datasize : Nat) (e
     (pure loop_vars) ) : Id (Int × Int × (BitVec datasize) × Bool) )
   (pure result)
 
-/-- Type quantifiers: k_ex18968_ : Bool, datasize : Nat, elements : Nat, esize : Nat, esize ≥ 1
+/-- Type quantifiers: k_ex22360_ : Bool, datasize : Nat, elements : Nat, esize : Nat, esize ≥ 1
   ∧ elements ≥ 1 ∧ (elements * esize) = datasize -/
 def vector_arithmetic_binary_uniform_cmp_bitwise (and_test : Bool) (datasize : Nat) (elements : Nat) (esize : Nat) (operand1 : (BitVec datasize)) (operand2 : (BitVec datasize)) : (BitVec datasize) := Id.run do
   let result : (BitVec datasize) := (Zeros datasize)
@@ -492,7 +492,7 @@ def vector_arithmetic_unary_cmp_int_bulk (comparison : CompareOp) (datasize : Na
     (pure loop_vars) ) : Id (Int × (BitVec datasize) × Bool) )
   (pure result)
 
-/-- Type quantifiers: k_ex19097_ : Bool, datasize : Nat, elements : Nat, esize : Nat, esize ≥ 1
+/-- Type quantifiers: k_ex22489_ : Bool, datasize : Nat, elements : Nat, esize : Nat, esize ≥ 1
   ∧ elements ≥ 1 ∧ (elements * esize) = datasize -/
 def vector_arithmetic_binary_uniform_sub_saturating (datasize : Nat) (elements : Nat) (esize : Nat) (operand1 : (BitVec datasize)) (operand2 : (BitVec datasize)) (is_unsigned : Bool) : (BitVec datasize) := Id.run do
   let result : (BitVec datasize) := (Zeros datasize)
@@ -515,7 +515,7 @@ def vector_arithmetic_binary_uniform_sub_saturating (datasize : Nat) (elements :
     (pure loop_vars) ) : Id (Int × Int × Int × (BitVec datasize)) )
   (pure result)
 
-/-- Type quantifiers: k_ex19148_ : Bool, shift : Int, k_ex19146_ : Bool, k_ex19145_ : Bool, datasize
+/-- Type quantifiers: k_ex22540_ : Bool, shift : Int, k_ex22538_ : Bool, k_ex22537_ : Bool, datasize
   : Nat, elements : Nat, esize : Nat, esize ≥ 1 ∧
   elements ≥ 1 ∧ (elements * esize) = datasize -/
 def vector_shift_right (accumulate : Bool) (datasize : Nat) (elements : Nat) (esize : Nat) (operand : (BitVec datasize)) (accumulator : (BitVec datasize)) (round : Bool) (shift : Int) (is_unsigned : Bool) : (BitVec datasize) := Id.run do
@@ -545,7 +545,7 @@ def vector_shift_right (accumulate : Bool) (datasize : Nat) (elements : Nat) (es
     (pure loop_vars) ) : Id (Int × (BitVec datasize)) )
   (pure result)
 
-/-- Type quantifiers: k_ex19201_ : Bool, datasize : Nat, elements : Nat, elements ≥ 1 ∧
+/-- Type quantifiers: k_ex22593_ : Bool, datasize : Nat, elements : Nat, elements ≥ 1 ∧
   (elements * 8) = datasize ∧ datasize ≤ 128 -/
 def vector_transfer_vector_table (datasize : Nat) (elements : Nat) (is_tbl : Bool) (indices : (BitVec datasize)) (table : (BitVec 128)) (dst : (BitVec datasize)) : (BitVec datasize) := Id.run do
   let result : (BitVec datasize) :=
@@ -569,7 +569,7 @@ def vector_transfer_vector_extract (datasize : Nat) (hi : (BitVec datasize)) (lo
   let concat : (BitVec (2 * datasize)) := (hi +++ lo)
   (BitVec.slice concat position datasize)
 
-/-- Type quantifiers: k_ex19233_ : Bool, k_ex19232_ : Bool, datasize : Nat, elements : Nat, esize :
+/-- Type quantifiers: k_ex22625_ : Bool, k_ex22624_ : Bool, datasize : Nat, elements : Nat, esize :
   Nat, esize ≥ 1 ∧ elements ≥ 1 ∧ (elements * esize) = datasize -/
 def vector_reduce_intmax (datasize : Nat) (elements : Nat) (esize : Nat) (operand : (BitVec datasize)) (min : Bool) (is_unsigned : Bool) : (BitVec esize) := Id.run do
   let maxmin : Int := 0
@@ -625,7 +625,7 @@ def num_of_LogicalOp (arg_ : LogicalOp) : Int :=
   | .LogicalOp_EOR => 1
   | .LogicalOp_ORR => 2
 
-/-- Type quantifiers: k_ex19291_ : Bool, datasize : Nat, datasize ≥ 1 -/
+/-- Type quantifiers: k_ex22683_ : Bool, datasize : Nat, datasize ≥ 1 -/
 def vector_arithmetic_binary_uniform_logical_andorr (datasize : Nat) (invert : Bool) (operand1 : (BitVec datasize)) (operand2__arg : (BitVec datasize)) (op : LogicalOp) : (BitVec datasize) :=
   let operand2 : (BitVec datasize) := operand2__arg
   let result : (BitVec datasize) := (Zeros datasize)
@@ -698,7 +698,7 @@ def FPNeg (op : (BitVec k_N)) : (BitVec k_N) :=
 def FPAbs (op : (BitVec k_N)) : (BitVec k_N) :=
   (0#1 +++ (BitVec.slice op 0 ((Sail.BitVec.length op) -i 1)))
 
-/-- Type quantifiers: k_ex19450_ : Bool, datasize : Nat, elements : Nat, esize : Nat, esize ∈
+/-- Type quantifiers: k_ex22842_ : Bool, datasize : Nat, elements : Nat, esize : Nat, esize ∈
   {32, 64} ∧ elements ≥ 1 ∧ (elements * esize) = datasize -/
 def vector_arithmetic_binary_uniform_add_fp (datasize : Nat) (elements : Nat) (esize : Nat) (operand1 : (BitVec datasize)) (operand2 : (BitVec datasize)) (fpcr : (BitVec 32)) (pair : Bool) : (BitVec datasize) := Id.run do
   let result : (BitVec datasize) := (Zeros datasize)
@@ -728,7 +728,7 @@ def vector_arithmetic_binary_uniform_add_fp (datasize : Nat) (elements : Nat) (e
     (pure loop_vars) ) : Id ((BitVec esize) × (BitVec esize) × (BitVec datasize)) )
   (pure result)
 
-/-- Type quantifiers: k_ex19557_ : Bool, datasize : Nat, elements : Nat, esize : Nat, esize ∈
+/-- Type quantifiers: k_ex22949_ : Bool, datasize : Nat, elements : Nat, esize : Nat, esize ∈
   {32, 64} ∧ elements ≥ 1 ∧ (elements * esize) = datasize -/
 def vector_arithmetic_binary_uniform_sub_fp (datasize : Nat) (elements : Nat) (esize : Nat) (operand1 : (BitVec datasize)) (operand2 : (BitVec datasize)) (fpcr : (BitVec 32)) (abs : Bool) : (BitVec datasize) := Id.run do
   let result : (BitVec datasize) := (Zeros datasize)
@@ -776,7 +776,7 @@ def vector_arithmetic_binary_uniform_mul_fp_product (datasize : Nat) (elements :
     (pure loop_vars) ) : Id ((BitVec esize) × (BitVec esize) × (BitVec datasize)) )
   (pure result)
 
-/-- Type quantifiers: k_ex19731_ : Bool, datasize : Nat, elements : Nat, esize : Nat, esize ∈
+/-- Type quantifiers: k_ex23123_ : Bool, datasize : Nat, elements : Nat, esize : Nat, esize ∈
   {32, 64} ∧ elements ≥ 1 ∧ (elements * esize) = datasize -/
 def vector_arithmetic_binary_uniform_mul_fp_fused (datasize : Nat) (elements : Nat) (esize : Nat) (operand1 : (BitVec datasize)) (operand2 : (BitVec datasize)) (operand3 : (BitVec datasize)) (fpcr : (BitVec 32)) (sub_op : Bool) : (BitVec datasize) := Id.run do
   let result : (BitVec datasize) := (Zeros datasize)
@@ -802,7 +802,7 @@ def vector_arithmetic_binary_uniform_mul_fp_fused (datasize : Nat) (elements : N
     (pure loop_vars) ) : Id ((BitVec esize) × (BitVec esize) × (BitVec datasize)) )
   (pure result)
 
-/-- Type quantifiers: k_ex19807_ : Bool, k_ex19806_ : Bool, datasize : Nat, elements : Nat, esize :
+/-- Type quantifiers: k_ex23199_ : Bool, k_ex23198_ : Bool, datasize : Nat, elements : Nat, esize :
   Nat, esize ∈ {32, 64} ∧ elements ≥ 1 ∧ (elements * esize) = datasize -/
 def vector_arithmetic_binary_uniform_maxmin_fp_1985 (datasize : Nat) (elements : Nat) (esize : Nat) (operand1 : (BitVec datasize)) (operand2 : (BitVec datasize)) (fpcr : (BitVec 32)) (minimum : Bool) (pair : Bool) : (BitVec datasize) := Id.run do
   let result : (BitVec datasize) := (Zeros datasize)
@@ -834,7 +834,7 @@ def vector_arithmetic_binary_uniform_maxmin_fp_1985 (datasize : Nat) (elements :
     (pure loop_vars) ) : Id ((BitVec esize) × (BitVec esize) × (BitVec datasize)) )
   (pure result)
 
-/-- Type quantifiers: k_ex19905_ : Bool, k_ex19904_ : Bool, datasize : Nat, elements : Nat, esize :
+/-- Type quantifiers: k_ex23297_ : Bool, k_ex23296_ : Bool, datasize : Nat, elements : Nat, esize :
   Nat, esize ∈ {32, 64} ∧ elements ≥ 1 ∧ (elements * esize) = datasize -/
 def vector_arithmetic_binary_uniform_maxmin_fp_2008 (datasize : Nat) (elements : Nat) (esize : Nat) (operand1 : (BitVec datasize)) (operand2 : (BitVec datasize)) (fpcr : (BitVec 32)) (minimum : Bool) (pair : Bool) : (BitVec datasize) := Id.run do
   let result : (BitVec datasize) := (Zeros datasize)
@@ -884,7 +884,7 @@ def vector_arithmetic_unary_special_sqrt (datasize : Nat) (elements : Nat) (esiz
     (pure loop_vars) ) : Id ((BitVec esize) × (BitVec datasize)) )
   (pure result)
 
-/-- Type quantifiers: k_ex20052_ : Bool, datasize : Nat, elements : Nat, esize : Nat, esize ∈
+/-- Type quantifiers: k_ex23444_ : Bool, datasize : Nat, elements : Nat, esize : Nat, esize ∈
   {32, 64} ∧ elements ≥ 1 ∧ (elements * esize) = datasize -/
 def vector_arithmetic_unary_diffneg_fp (datasize : Nat) (elements : Nat) (esize : Nat) (operand : (BitVec datasize)) (neg : Bool) : (BitVec datasize) := Id.run do
   let result : (BitVec datasize) := (Zeros datasize)
@@ -1150,6 +1150,43 @@ def num_of_SystemRegisterWriteTarget (arg_ : SystemRegisterWriteTarget) : Int :=
   | .SystemRegisterWriteTarget_SPSR_EL2 => 6
   | .SystemRegisterWriteTarget_HCR_EL2 => 7
 
+def system_register_cold_entry_target_pure (o0 : (BitVec 1)) (op1 : (BitVec 3)) (CRn : (BitVec 4)) (CRm : (BitVec 4)) (op2 : (BitVec 3)) (Rt : (BitVec 5)) : (Bool × SystemRegisterWriteTarget × (BitVec 5)) :=
+  if (((o0 == 1#1) && ((op1 == 0b100#3) && ((CRn == 0x1#4) && ((CRm == 0x1#4) && (op2 == 0b000#3))))) : Bool)
+  then (true, SystemRegisterWriteTarget_HCR_EL2, Rt)
+  else
+    (if (((o0 == 1#1) && ((op1 == 0b100#3) && ((CRn == 0x2#4) && ((CRm == 0x1#4) && (op2 == 0b000#3))))) : Bool)
+    then (true, SystemRegisterWriteTarget_VTTBR_EL2, Rt)
+    else
+      (if (((o0 == 1#1) && ((op1 == 0b100#3) && ((CRn == 0x2#4) && ((CRm == 0x1#4) && (op2 == 0b010#3))))) : Bool)
+      then (true, SystemRegisterWriteTarget_VTCR_EL2, Rt)
+      else
+        (if (((o0 == 1#1) && ((op1 == 0b100#3) && ((CRn == 0xE#4) && ((CRm == 0x1#4) && (op2 == 0b000#3))))) : Bool)
+        then (true, SystemRegisterWriteTarget_CNTHCTL_EL2, Rt)
+        else
+          (if (((o0 == 1#1) && ((op1 == 0b100#3) && ((CRn == 0xE#4) && ((CRm == 0x0#4) && (op2 == 0b011#3))))) : Bool)
+          then (true, SystemRegisterWriteTarget_CNTVOFF_EL2, Rt)
+          else
+            (if (((o0 == 1#1) && ((op1 == 0b100#3) && ((CRn == 0x4#4) && ((CRm == 0x1#4) && (op2 == 0b000#3))))) : Bool)
+            then (true, SystemRegisterWriteTarget_SP_EL1, Rt)
+            else
+              (if (((o0 == 1#1) && ((op1 == 0b100#3) && ((CRn == 0x4#4) && ((CRm == 0x0#4) && (op2 == 0b001#3))))) : Bool)
+              then (true, SystemRegisterWriteTarget_ELR_EL2, Rt)
+              else
+                (if (((o0 == 1#1) && ((op1 == 0b100#3) && ((CRn == 0x4#4) && ((CRm == 0x0#4) && (op2 == 0b000#3))))) : Bool)
+                then (true, SystemRegisterWriteTarget_SPSR_EL2, Rt)
+                else (false, SystemRegisterWriteTarget_HCR_EL2, Rt))))))))
+
+def decode64_cold_entry_system_write_pure (op_code : (BitVec 32)) : (Bool × SystemRegisterWriteTarget × (BitVec 5)) :=
+  let Rt : (BitVec 5) := (BitVec.slice op_code 0 5)
+  let op2 : (BitVec 3) := (BitVec.slice op_code 5 3)
+  let CRm : (BitVec 4) := (BitVec.slice op_code 8 4)
+  let CRn : (BitVec 4) := (BitVec.slice op_code 12 4)
+  let op1 : (BitVec 3) := (BitVec.slice op_code 16 3)
+  let o0 : (BitVec 1) := (BitVec.slice op_code 19 1)
+  if (((op_code &&& 0xFFF00000#32) == 0xD5100000#32) : Bool)
+  then (system_register_cold_entry_target_pure o0 op1 CRn CRm op2 Rt)
+  else (false, SystemRegisterWriteTarget_HCR_EL2, Rt)
+
 def system_register_vttbr_el2_target_pure (o0 : (BitVec 1)) (op1 : (BitVec 3)) (CRn : (BitVec 4)) (CRm : (BitVec 4)) (op2 : (BitVec 3)) (Rt : (BitVec 5)) : (Bool × SystemRegisterWriteTarget × (BitVec 5)) :=
   if (((o0 == 1#1) && ((op1 == 0b100#3) && ((CRn == 0x2#4) && ((CRm == 0x1#4) && (op2 == 0b000#3))))) : Bool)
   then (true, SystemRegisterWriteTarget_VTTBR_EL2, Rt)
@@ -1166,8 +1203,8 @@ def decode64_system_write_vttbr_el2_pure (op_code : (BitVec 32)) : (Bool × Syst
   then (system_register_vttbr_el2_target_pure o0 op1 CRn CRm op2 Rt)
   else (false, SystemRegisterWriteTarget_VTTBR_EL2, Rt)
 
-/-- Type quantifiers: k_ex20459_ : Bool, k_ex20458_ : Bool, k_ex20457_ : Bool, k_ex20456_ : Bool, k_ex20455_
-  : Bool, k_ex20454_ : Bool -/
+/-- Type quantifiers: k_ex24287_ : Bool, k_ex24286_ : Bool, k_ex24285_ : Bool, k_ex24284_ : Bool, k_ex24283_
+  : Bool, k_ex24282_ : Bool -/
 def aarch64_sysregwrite_vttbr_el2_pure (at_el1 : Bool) (hcr_nv : Bool) (hcr_nv2 : Bool) (hcr_tge : Bool) (scr_ns : Bool) (scr_eel2 : Bool) (old_value : (BitVec 64)) (val_name : (BitVec 64)) : (Bool × (BitVec 64)) :=
   let redirected : Bool :=
     (at_el1 && (hcr_nv && (hcr_nv2 && ((! hcr_tge) && (scr_ns || scr_eel2)))))
@@ -1191,8 +1228,8 @@ def decode64_system_write_vtcr_el2_pure (op_code : (BitVec 32)) : (Bool × Syste
   then (system_register_vtcr_el2_target_pure o0 op1 CRn CRm op2 Rt)
   else (false, SystemRegisterWriteTarget_VTCR_EL2, Rt)
 
-/-- Type quantifiers: k_ex20581_ : Bool, k_ex20580_ : Bool, k_ex20579_ : Bool, k_ex20578_ : Bool, k_ex20577_
-  : Bool, k_ex20576_ : Bool -/
+/-- Type quantifiers: k_ex24409_ : Bool, k_ex24408_ : Bool, k_ex24407_ : Bool, k_ex24406_ : Bool, k_ex24405_
+  : Bool, k_ex24404_ : Bool -/
 def aarch64_sysregwrite_vtcr_el2_pure (at_el1 : Bool) (hcr_nv : Bool) (hcr_nv2 : Bool) (hcr_tge : Bool) (scr_ns : Bool) (scr_eel2 : Bool) (old_value : (BitVec 32)) (val_name : (BitVec 64)) : (Bool × (BitVec 32)) :=
   let redirected : Bool :=
     (at_el1 && (hcr_nv && (hcr_nv2 && ((! hcr_tge) && (scr_ns || scr_eel2)))))
@@ -1235,8 +1272,8 @@ def decode64_system_write_cntvoff_el2_pure (op_code : (BitVec 32)) : (Bool × Sy
   then (system_register_cntvoff_el2_target_pure o0 op1 CRn CRm op2 Rt)
   else (false, SystemRegisterWriteTarget_CNTVOFF_EL2, Rt)
 
-/-- Type quantifiers: k_ex20817_ : Bool, k_ex20816_ : Bool, k_ex20815_ : Bool, k_ex20814_ : Bool, k_ex20813_
-  : Bool, k_ex20812_ : Bool -/
+/-- Type quantifiers: k_ex24645_ : Bool, k_ex24644_ : Bool, k_ex24643_ : Bool, k_ex24642_ : Bool, k_ex24641_
+  : Bool, k_ex24640_ : Bool -/
 def aarch64_sysregwrite_cntvoff_el2_pure (at_el1 : Bool) (hcr_nv : Bool) (hcr_nv2 : Bool) (hcr_tge : Bool) (scr_ns : Bool) (scr_eel2 : Bool) (old_value : (BitVec 64)) (val_name : (BitVec 64)) : (Bool × (BitVec 64)) :=
   let redirected : Bool :=
     (at_el1 && (hcr_nv && (hcr_nv2 && ((! hcr_tge) && (scr_ns || scr_eel2)))))
@@ -1260,8 +1297,8 @@ def decode64_system_write_sp_el1_pure (op_code : (BitVec 32)) : (Bool × SystemR
   then (system_register_sp_el1_target_pure o0 op1 CRn CRm op2 Rt)
   else (false, SystemRegisterWriteTarget_SP_EL1, Rt)
 
-/-- Type quantifiers: k_ex20939_ : Bool, k_ex20938_ : Bool, k_ex20937_ : Bool, k_ex20936_ : Bool, k_ex20935_
-  : Bool, k_ex20934_ : Bool -/
+/-- Type quantifiers: k_ex24767_ : Bool, k_ex24766_ : Bool, k_ex24765_ : Bool, k_ex24764_ : Bool, k_ex24763_
+  : Bool, k_ex24762_ : Bool -/
 def aarch64_sysregwrite_sp_el1_pure (at_el1 : Bool) (hcr_nv : Bool) (hcr_nv2 : Bool) (hcr_tge : Bool) (scr_ns : Bool) (scr_eel2 : Bool) (old_value : (BitVec 64)) (val_name : (BitVec 64)) : (Bool × (BitVec 64)) :=
   let redirected : Bool :=
     (at_el1 && (hcr_nv && (hcr_nv2 && ((! hcr_tge) && (scr_ns || scr_eel2)))))
@@ -1323,14 +1360,88 @@ def decode64_system_write_hcr_el2_pure (op_code : (BitVec 32)) : (Bool × System
   then (system_register_hcr_el2_target_pure o0 op1 CRn CRm op2 Rt)
   else (false, SystemRegisterWriteTarget_HCR_EL2, Rt)
 
-/-- Type quantifiers: k_ex21289_ : Bool, k_ex21288_ : Bool, k_ex21287_ : Bool, k_ex21286_ : Bool, k_ex21285_
-  : Bool, k_ex21284_ : Bool -/
+/-- Type quantifiers: k_ex25117_ : Bool, k_ex25116_ : Bool, k_ex25115_ : Bool, k_ex25114_ : Bool, k_ex25113_
+  : Bool, k_ex25112_ : Bool -/
 def aarch64_sysregwrite_hcr_el2_pure (at_el1 : Bool) (old_hcr_nv : Bool) (old_hcr_nv2 : Bool) (old_hcr_tge : Bool) (scr_ns : Bool) (scr_eel2 : Bool) (old_value : (BitVec 64)) (val_name : (BitVec 64)) : (Bool × (BitVec 64)) :=
   let redirected : Bool :=
     (at_el1 && (old_hcr_nv && (old_hcr_nv2 && ((! old_hcr_tge) && (scr_ns || scr_eel2)))))
   if (redirected : Bool)
   then (true, old_value)
   else (false, val_name)
+
+def undefined_ColdEntryRegisterState (_ : Unit) : SailM ColdEntryRegisterState := do
+  (pure { hcr_el2 := ← (undefined_bitvector 64)
+          vttbr_el2 := ← (undefined_bitvector 64)
+          vtcr_el2 := ← (undefined_bitvector 32)
+          cnthctl_el2 := ← (undefined_bitvector 32)
+          cntvoff_el2 := ← (undefined_bitvector 64)
+          sp_el1 := ← (undefined_bitvector 64)
+          elr_el2 := ← (undefined_bitvector 64)
+          spsr_el2 := ← (undefined_bitvector 32) })
+
+def undefined_ColdEntryRegisterInputs (_ : Unit) : SailM ColdEntryRegisterInputs := do
+  (pure { hcr_el2 := ← (undefined_bitvector 64)
+          vttbr_el2 := ← (undefined_bitvector 64)
+          vtcr_el2 := ← (undefined_bitvector 64)
+          cnthctl_el2 := ← (undefined_bitvector 64)
+          cntvoff_el2 := ← (undefined_bitvector 64)
+          sp_el1 := ← (undefined_bitvector 64)
+          elr_el2 := ← (undefined_bitvector 64)
+          spsr_el2 := ← (undefined_bitvector 64) })
+
+def undefined_ColdEntryRegisterSequenceResult (_ : Unit) : SailM ColdEntryRegisterSequenceResult := do
+  (pure { state := ← (undefined_ColdEntryRegisterState ())
+          write0 := ← (undefined_SystemRegisterWriteTarget ())
+          write1 := ← (undefined_SystemRegisterWriteTarget ())
+          write2 := ← (undefined_SystemRegisterWriteTarget ())
+          write3 := ← (undefined_SystemRegisterWriteTarget ())
+          write4 := ← (undefined_SystemRegisterWriteTarget ())
+          write5 := ← (undefined_SystemRegisterWriteTarget ())
+          write6 := ← (undefined_SystemRegisterWriteTarget ())
+          write7 := ← (undefined_SystemRegisterWriteTarget ()) })
+
+/-- Type quantifiers: k_ex25137_ : Bool, k_ex25136_ : Bool -/
+def aarch64_cold_entry_register_sequence_at_el2_pure (old_state : ColdEntryRegisterState) (inputs : ColdEntryRegisterInputs) (scr_ns : Bool) (scr_eel2 : Bool) : ColdEntryRegisterSequenceResult :=
+  let old_hcr_nv : Bool := ((BitVec.access old_state.hcr_el2 42) == 1#1)
+  let old_hcr_nv2 : Bool := ((BitVec.access old_state.hcr_el2 45) == 1#1)
+  let old_hcr_tge : Bool := ((BitVec.access old_state.hcr_el2 27) == 1#1)
+  let (_, hcr_el2) :=
+    (aarch64_sysregwrite_hcr_el2_pure false old_hcr_nv old_hcr_nv2 old_hcr_tge scr_ns scr_eel2
+      old_state.hcr_el2 inputs.hcr_el2)
+  let hcr_nv : Bool := ((BitVec.access hcr_el2 42) == 1#1)
+  let hcr_nv2 : Bool := ((BitVec.access hcr_el2 45) == 1#1)
+  let hcr_tge : Bool := ((BitVec.access hcr_el2 27) == 1#1)
+  let (_, vttbr_el2) :=
+    (aarch64_sysregwrite_vttbr_el2_pure false hcr_nv hcr_nv2 hcr_tge scr_ns scr_eel2
+      old_state.vttbr_el2 inputs.vttbr_el2)
+  let (_, vtcr_el2) :=
+    (aarch64_sysregwrite_vtcr_el2_pure false hcr_nv hcr_nv2 hcr_tge scr_ns scr_eel2
+      old_state.vtcr_el2 inputs.vtcr_el2)
+  let cnthctl_el2 := (aarch64_sysregwrite_cnthctl_el2_pure inputs.cnthctl_el2)
+  let (_, cntvoff_el2) :=
+    (aarch64_sysregwrite_cntvoff_el2_pure false hcr_nv hcr_nv2 hcr_tge scr_ns scr_eel2
+      old_state.cntvoff_el2 inputs.cntvoff_el2)
+  let (_, sp_el1) :=
+    (aarch64_sysregwrite_sp_el1_pure false hcr_nv hcr_nv2 hcr_tge scr_ns scr_eel2 old_state.sp_el1
+      inputs.sp_el1)
+  let elr_el2 := (aarch64_sysregwrite_elr_el2_pure inputs.elr_el2)
+  let spsr_el2 := (aarch64_sysregwrite_spsr_el2_pure inputs.spsr_el2)
+  { state := { hcr_el2 := hcr_el2
+               vttbr_el2 := vttbr_el2
+               vtcr_el2 := vtcr_el2
+               cnthctl_el2 := cnthctl_el2
+               cntvoff_el2 := cntvoff_el2
+               sp_el1 := sp_el1
+               elr_el2 := elr_el2
+               spsr_el2 := spsr_el2 }
+    write0 := SystemRegisterWriteTarget_HCR_EL2
+    write1 := SystemRegisterWriteTarget_VTTBR_EL2
+    write2 := SystemRegisterWriteTarget_VTCR_EL2
+    write3 := SystemRegisterWriteTarget_CNTHCTL_EL2
+    write4 := SystemRegisterWriteTarget_CNTVOFF_EL2
+    write5 := SystemRegisterWriteTarget_SP_EL1
+    write6 := SystemRegisterWriteTarget_ELR_EL2
+    write7 := SystemRegisterWriteTarget_SPSR_EL2 }
 
 def initialize_registers (_ : Unit) : Unit :=
   ()
